Datalog/Available_Expressions.thy
@@ -50,18 +50,18 @@ locale analysis_AE = finite_program_graph pg
   for pg :: "('n::finite,'v::finite action) program_graph"
 begin
 
-interpretation LTS edge_set .
+interpretation LTS edges .
 
 definition analysis_dom_AE :: "'v arith set" where
   "analysis_dom_AE = aexp_pg pg"
 
 lemma finite_analysis_dom_AE: "finite analysis_dom_AE"
 proof -
-  have "finite (\<Union> (aexp_edge ` edge_set))"
+  have "finite (\<Union> (aexp_edge ` edges))"
     by (metis aexp_edge.elims finite_UN finite_aexp_edge finite_program_graph_axioms 
         finite_program_graph_def)
   then show ?thesis
-    unfolding analysis_dom_AE_def using edge_set_def by force 
+    unfolding analysis_dom_AE_def using edges_def by force 
 qed
 
 fun kill_set_AE :: "('n,'v action) edge \<Rightarrow> 'v arith set" where
@@ -286,7 +286,7 @@ proof -
   from assms have "fw_must.summarizes_fw_must \<rho>"
     using fw_must.sound_ana_pg_fw_must by auto
   then show ?thesis
-    unfolding summarizes_AE_def fw_must.summarizes_fw_must_def edge_set_def edge_set_def
+    unfolding summarizes_AE_def fw_must.summarizes_fw_must_def edges_def edges_def
       end_def end_def aexp_path_S_hat_path_iff start_def start_def by force
 qed
 
