Datalog/Bit_Vector_Framework.thy
@@ -116,7 +116,7 @@ begin
 lemma finite_d_init: "finite d_init"
   by (meson analysis_BV_forward_may_axioms analysis_BV_forward_may_axioms_def analysis_BV_forward_may_def rev_finite_subset)
 
-interpretation LTS edge_set .
+interpretation LTS edges .
 
 definition "S_hat" :: "('n,'a) edge \<Rightarrow> 'd set \<Rightarrow> 'd set" ("S^\<^sub>E\<lbrakk>_\<rbrakk> _") where
   "S^\<^sub>E\<lbrakk>e\<rbrakk> R = (R - kill_set e) \<union> gen_set e"
@@ -221,11 +221,11 @@ proof -
 qed
 
 definition ana_pg_fw_may :: "(pred, var, ('n, 'a, 'd) cst) clause set" where
-  "ana_pg_fw_may = \<Union>(ana_edge ` edge_set)
+  "ana_pg_fw_may = \<Union>(ana_edge ` edges)
                \<union> ana_init ` d_init
                \<union> ana_anadom ` analysis_dom
-               \<union> \<Union>(ana_kill_edge ` edge_set)
-               \<union> \<Union>(ana_gen_edge ` edge_set)
+               \<union> \<Union>(ana_kill_edge ` edges)
+               \<union> \<Union>(ana_gen_edge ` edges)
                \<union> ana_must ` UNIV
                \<union> {ana_entry_node}"
 
@@ -272,24 +272,24 @@ lemma ana_pg_fw_may_stratified: "strat_wf s_BV ana_pg_fw_may"
   unfolding ana_pg_fw_may_def strat_wf_def ana_init_def ana_anadom_def ana_gen_edge_def 
     ana_must_def ana_entry_node_def  ana_kill_edge_def by auto
 
-lemma finite_ana_edge_edgeset: "finite (\<Union> (ana_edge ` edge_set))"
+lemma finite_ana_edge_edgeset: "finite (\<Union> (ana_edge ` edges))"
 proof -
-  have "finite edge_set"
+  have "finite edges"
     using finite_program_graph_axioms finite_program_graph_def by blast
   moreover
-  have "\<forall>e \<in> edge_set. finite (ana_edge e)"
+  have "\<forall>e \<in> edges. finite (ana_edge e)"
     by force
   ultimately
   show ?thesis
     by blast
 qed
 
-lemma finite_ana_kill_edgeset: "finite (\<Union> (ana_kill_edge ` edge_set))"
+lemma finite_ana_kill_edgeset: "finite (\<Union> (ana_kill_edge ` edges))"
 proof -
-  have "finite edge_set"
+  have "finite edges"
     using finite_program_graph_axioms finite_program_graph_def by blast
   moreover
-  have "\<forall>e \<in> edge_set. finite (ana_kill_edge e)"
+  have "\<forall>e \<in> edges. finite (ana_kill_edge e)"
     by (metis ana_kill_edge_def analysis_BV_forward_may_axioms analysis_BV_forward_may_axioms_def 
         analysis_BV_forward_may_def finite_Int finite_imageI kill_set_eq_kill_set_inter_analysis_dom)
   ultimately
@@ -297,12 +297,12 @@ proof -
     by blast
 qed
 
-lemma finite_ana_gen_edgeset: "finite (\<Union> (ana_gen_edge ` edge_set))"
+lemma finite_ana_gen_edgeset: "finite (\<Union> (ana_gen_edge ` edges))"
 proof -
-  have "finite edge_set"
+  have "finite edges"
     using finite_program_graph_axioms finite_program_graph_def by blast
   moreover
-  have "\<forall>e \<in> edge_set. finite (ana_gen_edge e)"
+  have "\<forall>e \<in> edges. finite (ana_gen_edge e)"
     by (metis ana_gen_edge_def analysis_BV_forward_may_axioms analysis_BV_forward_may_axioms_def 
         analysis_BV_forward_may_def finite_imageI rev_finite_subset)
   ultimately
@@ -387,7 +387,7 @@ lemma S_hat_path_last:
 
 lemma gen_sound:
   assumes "d \<in> gen_set (q, \<alpha>, q')"
-  assumes "(q, \<alpha>, q') \<in> edge_set"
+  assumes "(q, \<alpha>, q') \<in> edges"
   assumes "\<rho> \<Turnstile>\<^sub>l\<^sub>s\<^sub>t ana_pg_fw_may s_BV"
   shows "\<rho> \<Turnstile>\<^sub>c\<^sub>l\<^sub>s gen\<langle>[Cst\<^sub>N q, Cst\<^sub>A \<alpha>, Cst\<^sub>N q', Cst\<^sub>E d]\<rangle> :- [] ."
 proof -
@@ -492,7 +492,7 @@ locale analysis_BV_backward_may = finite_program_graph pg
   fixes kill_set :: "('n,'a) edge \<Rightarrow> 'd set"
   fixes gen_set :: "('n,'a) edge \<Rightarrow> 'd set"
   fixes d_init :: "'d set"
-  assumes "finite edge_set"
+  assumes "finite edges"
   assumes "finite analysis_dom"
   assumes "d_init \<subseteq> analysis_dom"
   assumes "\<forall>e. gen_set e \<subseteq> analysis_dom"
@@ -501,7 +501,7 @@ begin
 
 
 
-interpretation LTS edge_set .
+interpretation LTS edges .
 
 definition S_hat :: "('n,'a) edge \<Rightarrow> 'd set \<Rightarrow> 'd set" ("S^\<^sub>E\<lbrakk>_\<rbrakk> _") where
   "S^\<^sub>E\<lbrakk>e\<rbrakk> R = (R - kill_set e) \<union> gen_set e"
@@ -562,7 +562,7 @@ lemma gen_subs_analysis_dom: "(gen_set (rev_edge e)) \<subseteq> analysis_dom"
 interpretation fw_may: analysis_BV_forward_may pg_rev analysis_dom "\<lambda>e. (kill_set (rev_edge e))" "(\<lambda>e. gen_set (rev_edge e))" d_init
   using analysis_BV_forward_may_def finite_pg_rev analysis_BV_backward_may_axioms analysis_BV_backward_may_def
   by (metis (no_types, lifting) analysis_BV_backward_may_axioms_def 
-      analysis_BV_forward_may_axioms_def finite_program_graph_def program_graph.edge_set_def)
+      analysis_BV_forward_may_axioms_def finite_program_graph_def program_graph.edges_def)
  
 abbreviation ana_pg_bw_may where
   "ana_pg_bw_may == fw_may.ana_pg_fw_may"
@@ -612,8 +612,8 @@ lemma summarizes_bw_may_forward_backward':
   assumes "fw_may.summarizes_fw_may \<rho>"
   shows "\<rho> \<Turnstile>\<^sub>l\<^sub>h may\<langle>[Cst\<^sub>N (start_of (ss, w)), Cst\<^sub>E d]\<rangle>."
 proof -
-  have rev_in_edge_set: "(rev ss, rev w) \<in> LTS.path_with_word fw_may.edge_set"
-    using assms(1) rev_path_in_rev_pg[of ss w] fw_may.edge_set_def pg_rev_def by auto 
+  have rev_in_edges: "(rev ss, rev w) \<in> LTS.path_with_word fw_may.edges"
+    using assms(1) rev_path_in_rev_pg[of ss w] fw_may.edges_def pg_rev_def by auto 
   moreover
   have "LTS.start_of (rev ss, rev w) = fw_may.start"
     using assms(1,2) rev_end_is_start by (metis LTS.path_with_word_not_empty)
@@ -666,7 +666,7 @@ lemma finite_d_init: "finite d_init"
   by (meson analysis_BV_forward_must.axioms(2) analysis_BV_forward_must_axioms 
       analysis_BV_forward_must_axioms_def rev_finite_subset)
 
-interpretation LTS edge_set .
+interpretation LTS edges .
 
 definition S_hat :: "('n,'a) edge \<Rightarrow> 'd set \<Rightarrow> 'd set" ("S^\<^sub>E\<lbrakk>_\<rbrakk> _") where
   "S^\<^sub>E\<lbrakk>e\<rbrakk> R = (R - kill_set e) \<union> gen_set e"
@@ -1286,8 +1286,8 @@ proof -
   have "\<not>the_Elem\<^sub>i\<^sub>d d \<in> fw_may.S_hat_path \<pi> (analysis_dom - d_init)"
     using fw_may.sound_ana_pg_fw_may assms(1)
     unfolding fw_may.summarizes_fw_may_def
-     edge_set_def start_def assms(2) edge_set_def start_def
-    using assms(3)  d_encdec edge_set_def not_may start_def by (metis (mono_tags) mem_Collect_eq) 
+     edges_def start_def assms(2) edges_def start_def
+    using assms(3)  d_encdec edges_def not_may start_def by (metis (mono_tags) mem_Collect_eq) 
   then show "the_Elem\<^sub>i\<^sub>d d \<in> S^\<^sub>P\<lbrakk>\<pi>\<rbrakk> d_init"
     using opposite_lemma_path
     using assms(1)
@@ -1318,7 +1318,7 @@ lemma finite_d_init: "finite d_init"
   by (meson analysis_BV_backward_must.axioms(2) analysis_BV_backward_must_axioms 
       analysis_BV_backward_must_axioms_def rev_finite_subset)
 
-interpretation LTS edge_set .
+interpretation LTS edges .
 
 definition S_hat :: "('n,'a) edge \<Rightarrow> 'd set \<Rightarrow> 'd set" ("S^\<^sub>E\<lbrakk>_\<rbrakk> _") where
   "S^\<^sub>E\<lbrakk>e\<rbrakk> R = (R - kill_set e) \<union> gen_set e"
@@ -1374,7 +1374,7 @@ interpretation fw_must: analysis_BV_forward_must pg_rev analysis_dom "\<lambda>e
   using analysis_BV_forward_must_def finite_pg_rev analysis_BV_backward_must_axioms
     analysis_BV_backward_must_def analysis_BV_backward_must_axioms_def
     analysis_BV_forward_must_axioms.intro finite_program_graph.intro
-    program_graph.edge_set_def by metis
+    program_graph.edges_def by metis
 
 
 abbreviation ana_pg_bw_must where
@@ -1450,12 +1450,12 @@ lemma summarizes_fw_must_forward_backward':
   shows "the_Elem\<^sub>i\<^sub>d d \<in> S^\<^sub>P\<lbrakk>\<pi>\<rbrakk> d_init"
 proof -
   define rev_\<pi> where "rev_\<pi> = (rev (fst \<pi>), rev (snd \<pi>))"
-  have rev_\<pi>_path: "rev_\<pi> \<in> LTS.path_with_word fw_must.edge_set"
-    using rev_\<pi>_def assms(3) fw_must.edge_set_def pg_rev_def rev_path_in_rev_pg
+  have rev_\<pi>_path: "rev_\<pi> \<in> LTS.path_with_word fw_must.edges"
+    using rev_\<pi>_def assms(3) fw_must.edges_def pg_rev_def rev_path_in_rev_pg
     by (metis (no_types, lifting) fst_conv mem_Collect_eq  prod.collapse)
   have rev_\<pi>_start: "start_of rev_\<pi> = fw_must.start"
     using  rev_\<pi>_def analysis_BV_backward_must_axioms
-      assms(3) pg_rev_def start_of_def edge_set_def end_of_def hd_rev  
+      assms(3) pg_rev_def start_of_def edges_def end_of_def hd_rev  
       by (metis (mono_tags, lifting) fw_must.start_def mem_Collect_eq prod.sel)
   have rev_\<pi>_start_end: "end_of rev_\<pi> = the_Node\<^sub>i\<^sub>d q"
     using assms(3) rev_\<pi>_def end_of_def last_rev start_of_def
